\documentclass[12pt]{article}
\usepackage{amsfonts}
\usepackage{amsmath}




\begin{document}

\begin{equation}
\begin{aligned}
	\mathbb{E}[ (y - \tilde y)^2 ] &= \mathbb{E}[(y - \mathbb{E}[\tilde y] + \mathbb{E}[\tilde y] - \tilde y )^2]
	\\
	& = \mathbb{E}[(y - \mathbb{E}[\tilde y])^2] + \mathbb{E}[(\mathbb{E}[\tilde y] - \tilde y)^2] + 2 \mathbb{E}[(\mathbb{E}[\tilde y] - \tilde y)(y - \mathbb{E}[\tilde y])]
	\\
%	\text{However, this the third term is equal to:}
	\\
\mathbb{E}[(\mathbb{E}[\tilde y] - \tilde y)(y - \mathbb{E}[\tilde y])] & = \mathbb{E}[\mathbb{E}[\tilde y]y - \mathbb{E}[\tilde y]^2 - \tilde y y + \tilde y \mathbb{E}[\tilde y]]
\\
& = ( \mathbb{E}[\tilde y]^2 - \mathbb{E}[\tilde y]^2 - \mathbb{E}[\tilde y] \mathbb{E}[\tilde y] + \mathbb{E}[\tilde y] \mathbb{E}[\tilde y] )
\\
	& =0
	\\
	\\
\mathbb{E}[ (y - \tilde y)^2 ]	& = 	\mathbb{E}[(f + \epsilon - \mathbb{E}[\tilde y])^2] + \mathbb{E}[(\tilde y - \mathbb{E}[\tilde y])^2]
	\\
	& = \mathbb{E}[f - \mathbb{E}[\tilde y])^2] + \mathbb{E}[\epsilon^2] + 2 \mathbb{E}[(\epsilon) (f - \mathbb{E}[\tilde y])^2)] + \mathbb{E}[(\tilde y -\mathbb{E}[\tilde y])^2]
	\\
	\\
\mathbb{E}[(\epsilon) (f - \mathbb{E}[\tilde y])^2)]	
	& = \mathbb{E}[(\epsilon)] \ \mathbb{E}[(f - \mathbb{E}[\tilde y])^2)]
	\\
	& = 0
	\\
	\\	
\mathbb{E}[ (y - \tilde y)^2 ]		& = \mathbb{E}[f - \mathbb{E}[\tilde y])^2] + \mathbb{E}[\epsilon^2] + \mathbb{E}[(\tilde y -\mathbb{E}[\tilde y])^2]
\\
& = Bias^2 + \sigma^2_\epsilon + Variance 
\end{aligned}
\end{equation}


\end{document}